theories/union_find/Proof.v
@@ -1,0 +1,1066 @@
+From TLC Require Import LibTactics LibLogic LibSet LibRelation LibFun LibEqual
+                        LibInt.
+From iris_time.union_find.math Require Import TLCBuffer.
+
+From stdpp Require Import gmap.
+
+From iris.bi Require Import big_op.
+From iris.heap_lang Require Import proofmode.
+From iris_time Require Import TimeCredits MachineIntegers.
+
+(* Load extra math libraries. *)
+From iris_time.union_find.math Require Import LibNatExtra InverseAckermann.
+(* Load the mathematical analysis of UnionFind. *)
+From iris_time.union_find.math Require Import UnionFind01Data
+     UnionFind02EmptyCreate UnionFind03Link UnionFind04Compress
+     UnionFind05IteratedCompression UnionFind06Join UnionFind11Rank
+     UnionFind12RankEmptyCreate UnionFind13RankLink UnionFind14RankCompress
+     UnionFind15RankJoin UnionFind41Potential UnionFind43PotentialAnalysis
+     UnionFind44PotentialJoin.
+
+(* Load the heap_lang code *)
+From iris_time.union_find Require Import Code.
+
+Section UnionFind.
+
+Context `{!timeCreditHeapG Σ}.
+
+(* An object in the Union Find data structure is represented by an
+   heap_lang location. *)
+Notation elem := loc.
+
+(* The logical type of the content of a vertex. *)
+Inductive content :=
+| Root : nat -> val -> content
+| Link : elem -> content.
+
+Definition val_of_content (c : content) : val :=
+  match c with
+  | Root k v => ROOTV(#k, v)
+  | Link e => LINKV #e
+  end.
+
+(* Hints for the type-checker. *)
+
+(* It seems important that [D], [R], and [V] which are the public parameters to
+   [UF], mention [elem] in their types, as opposed to [loc]. Internally [elem]
+   is equal to [loc]. Ultimately, however, the type [elem] is made opaque. *)
+
+Implicit Types x y r : elem.
+Implicit Types v : val.
+Implicit Types D : LibSet.set elem.  (* domain *)
+Implicit Types F : binary elem.      (* edges *)
+Implicit Types K : elem -> nat.      (* rank *)
+Implicit Types R : elem -> elem.     (* functional view of [is_repr F] *)
+Implicit Types V : elem -> val.      (* data stored at the roots *)
+Implicit Types M : gmap elem content. (* view of the memory *)
+
+(* -------------------------------------------------------------------------- *)
+
+(* Invariants and representation predicate. *)
+
+(* The predicate [Mem ...] relates the mathematical graph encoded by [D/F/K/V]
+   and the memory encoded by the finite map [M]. In short,
+    1. elements of [D] have a mapping in M;
+    2. the links in [M] coincide with the links in [F];
+    3. the rank and data stored at a root in [M] agree with [K] and [V]. *)
+
+Definition Mem D F K V M : Prop :=
+  forall x, x \in D ->
+    match M!!x with
+    | Some (Link y)   => F x y
+    | Some (Root k v) => is_root F x /\ k = K x /\ v = V x
+    | None => False
+    end.
+
+(* The predicate [Inv ...] relates the mathematical graph encoded by [D/F/K/V]
+   and the view that is exposed to the client, which is encoded by [D/R/V].
+   In short,
+   1. [D/F/K] form a ranked disjoint set forest, as per [is_rdsf];
+   2. [R] is included in [is_repr F],
+      which means that [R x = y] implies [is_repr F x y],
+      or in other words, [R] agrees with [F];
+   3. [V] agrees with [R]. *)
+
+Record Inv D F K R V : Prop := {
+  Inv_rdsf  : is_rdsf D F K;
+  Inv_incl  : fun_in_rel R (is_repr F);
+  Inv_data  : forall x, V x = V (R x)
+}.
+
+Hint Resolve is_rdsf_is_dsf.
+Hint Resolve Inv_rdsf Inv_incl Inv_data.
+
+(* Throughout, we instantiate the parameter [r] of Alstrup et al.'s proof
+   with the value 1. Thus, we write just [Phi] for [Phi 1]. *)
+
+Notation Phi := (Phi 1).
+
+(* [UF D R V] is the representation predicate. It is an abstract predicate: the
+   client uses this predicate, but does not know how it is defined. *)
+
+(* The definition asserts the existence (and ownership) of a group of references,
+   whose content is described by a finite map [M]. It asserts the two invariants
+   above. Finally, it asserts the existence (and ownership) of [Phi] time credits,
+   which have been set aside to help pay for future operations. The definition
+   quantifies existentially over [F/K/M], which therefore are not exposed to the
+   client. *)
+
+Definition mapsto_M M : iProp Σ :=
+  ([∗ map] l ↦ c ∈ M, l ↦ val_of_content c)%I.
+
+Definition UF D R V : iProp Σ :=
+  (∃ F K M,
+  ⌜ Inv D F K R V ⌝ ∗
+  ⌜ Mem D F K V M ⌝ ∗
+  mapsto_M M ∗
+  TC (7 * Phi D F K))%I.
+
+(* -------------------------------------------------------------------------- *)
+
+(* The functions [V] and [R] are compatible with [R]. In other words, every
+   member of an equivalence class must have the same image through [V] (see
+   [Inv_data]) and through [R]. For this reason, when we wish to update one of
+   these functions, we must update it not just at one point, but at a whole
+   equivalence class. *)
+
+(* The function [update1 R f x b] coincides with the function [f] everywhere,
+   except on the equivalence class of [x], whose elements are mapped to [b]. *)
+
+Definition update1 {B : Type} (f : elem -> B) R x (b : B) :=
+  fcupdate f (fun z => R z = R x) b.
+
+(* The function [update2 R f x y b] coincides with the function [f] everywhere,
+   except on the equivalence classes of [x] and [y], whose elements are mapped
+   to [b]. *)
+
+Definition update2 {B : Type} (f : elem -> B) R x y b :=
+  fcupdate f (fun z => R z = R x \/ R z = R y) b.
+
+(* Updating [V] by mapping the equivalence classes of [x] and [x] to [V x]
+   has no effect. *)
+
+Lemma update2_V_self : forall D F K R V x,
+  Inv D F K R V ->
+  update2 V R x x (V x) = V.
+Proof using.
+  introv [ _ _ H ]. unfold update2.
+  eapply fcupdate_self; intros.
+  branches; rewrite H; congruence.
+Qed.
+
+(* If [x] is a root, then updating [R] by mapping the equivalence classes of [x]
+   and [x] to [x] has no effect. *)
+
+Lemma update2_R_self : forall R x,
+  R x = x ->
+  update2 R R x x x = R.
+Proof using.
+  intros. unfold update2.
+  eapply fcupdate_self; intros.
+  branches; congruence.
+Qed.
+
+(* Updating [f] at [R x] and [R y] is the same as updating [f] at [x] and [y]. *)
+
+Lemma update2_root : forall (B : Type) (f : elem -> B) R x y b,
+  idempotent R ->
+  update2 f R (R x) (R y) b = update2 f R x y b.
+Proof using.
+  introv H. unfold update2. do 2 rewrite* H.
+Qed.
+
+(* Updating [V] at [x] and [y] is the same as updating [V] at [y] and [x]. *)
+
+Lemma update2_sym : forall B (f : elem -> B) R x y b,
+  update2 f R x y b = update2 f R y x b.
+Proof using.
+  intros. extens. intros z. unfold update2.
+  f_equal. clear z. extens; intros z. tauto.
+Qed.
+
+(* -------------------------------------------------------------------------- *)
+
+(* Exploitation and preservation lemmas for the invariant [Inv]. *)
+
+(* If [x] is in the domain and [r] is its representative, then [r] is in the
+   domain and [r] is its own representative. *)
+
+Lemma Inv_root : forall D F K R V x r,
+  Inv D F K R V ->
+  x \in D ->
+  r = R x ->
+  r \in D /\ R r = r.
+Proof using.
+  intros; subst; split.
+  applys* sticky_R.
+  applys* idempotent_R.
+Qed.
+
+(* The invariant is preserved when a new element [r] is created and the
+   function [V] is updated at [r] in an arbitrary manner. *)
+
+Lemma Inv_make : forall D R F K V D' V' r v,
+  Inv D F K R V ->
+  r \notin D ->
+  D' = D \u \{r} ->
+  V' = update1 V R r v ->
+  Inv D' F K R V'.
+Proof using.
+  introv HI Dr ED EV. subst D'. lets [Hrdsf Hroots Hdata]: HI.
+  constructor.
+  { eauto using is_rdsf_create. }
+  { auto. }
+  { subst V'. eapply fcupdate_absorbs; intros; eauto.
+    rewrites* (>> idempotent_R R). }
+Qed.
+
+(* The invariant is preserved by updating [V] at one equivalence class. *)
+
+Lemma Inv_update1 : forall D F K R V x v,
+  Inv D F K R V ->
+  Inv D F K R (update1 V R x v).
+Proof using.
+  introv [? ? ?]. constructors~; intros.
+  eapply fcupdate_absorbs; intros; eauto.
+  rewrites* (>> idempotent_R R).
+Qed.
+
+(* The invariant is preserved by a [link] operation. *)
+
+(* The hypothesis is that the invariant holds and [x] and [y] are distinct roots
+   in the domain. The conclusion is that the invariant holds again and the
+   potential [Phi] grows by at most 2. The domain [D] is unchanged, while the
+   other parameters [F'/K'/R'/V'/z] are described by five equations. *)
+
+Lemma Inv_link: forall D R F K V F' K' V' x y z,
+  (* Hypotheses: *)
+  Inv D F K R V ->
+  x ≠ y ->
+  x \in D ->
+  y \in D ->
+  R x = x ->
+  R y = y ->
+  (* Five equations, describing the situation after the link: *)
+  z = new_repr_by_rank K x y ->
+  F' = link_by_rank_F F K x y ->
+  K' = link_by_rank_K K x y ->
+  V' = update2 V R x y (V z) ->
+  let R' := link_by_rank_R R x y z in
+  (* Conclusions: *)
+  Inv D F' K' R' V' /\
+  (Phi D F' K' <= Phi D F K + 2)%nat.
+Proof.
+  introv HI. intros. subst R' F' K' V' z. split. constructor.
+  (* Preservation of [is_rdsf]. *)
+  { eauto 8 using is_rdsf_link, R_self_is_root. }
+  (* Preservation of the agreement between [R] and [F]. *)
+  { eauto 8 using link_by_rank_R_link_by_rank_F_agree, R_self_is_root. }
+  (* Preservation of the agreement between [V] and [R]. *)
+  { intros w.
+    unfold update2, fcupdate, link_by_rank_R. repeat case_if~.
+    { false. forwards* HR: idempotent_R R. rewrite ->HR in *. tauto. }
+    { rewrites~ <- (>> Inv_data HI). }
+  }
+  (* Change in potential. *)
+  { eapply potential_increase_during_link; eauto using R_self_is_root. }
+Qed.
+
+(* This tactic helps apply the above lemma. The user is supposed to supply
+   expressions for [F'/K'/V'/z], which we prove equal to what we expect.
+   This allows some flexibility. *)
+
+Ltac Inv_link F' K' V' x y z :=
+  match goal with HInv: Inv ?D ?F ?K ?R ?V |- _ =>
+    let Hpotential := fresh in
+    (* Apply [Inv_link] to appropriate parameters. *)
+    forwards* (?&Hpotential):
+      (Inv_link _ _ _ _ _ F' K' V' x y z HInv);
+    (* We expect to see some equations as sub-goals. We prove them by
+       unfolding definitions and performing a simple case analysis. *)
+    try solve [
+       unfold new_repr_by_rank, link_by_rank_F, link_by_rank_K;
+       case_if; solve [ eauto | math ]
+     | congruence
+    ]
+  end.
+
+(* -------------------------------------------------------------------------- *)
+
+(* Exploitation and preservation lemmas for the invariant [Mem]. *)
+
+(* If [x] is in the domain and is a root, then [M] maps [x] to [Root]
+   with rank [K x] and data [V x]. *)
+
+Lemma Mem_root : forall D R F K M V x,
+  Inv D F K R V ->
+  Mem D F K V M ->
+  x \in D ->
+  R x = x ->
+  M!!x = Some (Root (K x) (V x)).
+Proof using.
+  introv HI HM Dx Rxx.
+  forwards~ HV: HM x. destruct (M!!x) as [[]|]; [| |done].
+    destruct HV as (?&?&?). congruence.
+    false* (>> R_self_is_root HI HV).
+Qed.
+
+(* Conversely, if [M] maps [x] to [Root], then [x] is a root whose
+   rank and data are as predicted by [M]. *)
+
+Lemma Mem_root_inv : forall D F K M V x rx vx,
+  Mem D F K V M ->
+  x \in D ->
+  M!!x = Some(Root rx vx) ->
+  is_root F x /\ rx = K x /\ vx = V x.
+Proof using.
+  introv HM Dx HE. forwards~ HVx: HM x.
+  destruct (M!!x) as [[]|]; [|false|done]. inverts* HE.
+Qed.
+
+(* [Mem] is preserved when a new element [r] is created with rank 0 and the
+   function [V] is updated at [r] in an arbitrary manner. *)
+
+Lemma Mem_make : forall D R F K D' r M V v,
+  Inv D F K R V ->
+  Mem D F K V M ->
+  is_rdsf D F K ->
+  r \notin D ->
+  D' = D \u \{r} ->
+  Mem D' F K (update1 V R r v) (<[r:=Root 0 v]>M).
+Proof using.
+  introv HI HV HG Dr -> Dx.
+  rewrite in_union_eq in_single_eq in Dx. destruct Dx as [Dx| ->].
+  { rewrite lookup_insert_ne; [|naive_solver].
+    rewrite /update1 fcupdate_miss; [by apply HV|].
+    intro. forwards* : R_is_identity_outside_D R r.
+    forwards*: Inv_root x (R x). intuition congruence. }
+  { rewrite lookup_insert /update1 fcupdate_hit //. splits.
+    { eauto using only_roots_outside_D with is_dsf. }
+    { (* We use the fact that [K] is zero outside the domain. *)
+      erewrite is_rdsf_zero_rank_outside_domain; eauto. }
+    { done. } }
+Qed.
+
+(* [Mem] is preserved by installing a link from a root [x] to a root [y]
+   without updating any rank. *)
+
+Lemma Mem_link : forall D F R K F' M V V' x y,
+  Inv D F K R V ->
+  Mem D F K V M ->
+  x \in D ->
+  x = R x ->
+  y = R y ->
+  F' = UnionFind03Link.link F x y ->
+  V' = update2 V R x y (V y) ->
+  Mem D F' K V' (<[x:=Link y]>M).
+Proof using.
+  introv HI HR Dx Rx Ry EG' HV. subst F'.
+  intros a Da. specializes HR Da.
+  destruct (decide (x = a)) as [->|].
+  { rewrite lookup_insert. eauto using link_appears. }
+  rewrite lookup_insert_ne //. destruct (M!!a) as [[]|]; [| |done]; first last.
+  { eauto using link_previous. }
+  rewrite~ HV. destruct HR as (?&?&E). splits*.
+  { applys* is_root_link. }
+  rewrites (rm E).
+  unfold update2, fcupdate. rewrites <- (rm Rx). rewrites <- (rm Ry).
+  forwards* Ra: is_root_R_self a. rewrite Ra. case_if~.
+  branches. false. congruence.
+Qed.
+
+(* [Mem] is preserved by installing a link from a root [x] to a root [y]
+   and incrementing the rank of [y]. *)
+
+Lemma Mem_link_incr : forall D F R K F' K' M V V' x y (rx : nat) v,
+  Inv D F K R V ->
+  Mem D F K V M ->
+  x \in D ->
+  y \in D ->
+  x = R x ->
+  y = R y ->
+  x ≠ y ->
+  rx = K x ->
+  F' = UnionFind03Link.link F x y ->
+  K' = fupdate K y (1 + K x)%nat ->
+  v = V y ->
+  V' = update2 V R x y (V y) ->
+  Mem D F' K' V' (<[y:=Root (rx + 1) v]>(<[x:=Link y]>M)).
+Proof using.
+  introv HI HM Dx Dy Rx Ry HN Hy Kx HK. introv Hv HV'.
+  forwards* HV: (>> Mem_link V V' x y HM).
+  sets M': (<[x := Link y]>M). clearbody M'.
+  intros a Da. specializes HV Da. destruct (decide (y = a)) as [->|].
+  { rewrite lookup_insert. splits.
+    { subst F'. applys* is_root_link. applys* R_self_is_root. }
+    { subst K'. subst rx. rewrite fupdate_same. math. }
+    { subst v. subst V'. rewrite /update2 fcupdate_hit; by auto. } }
+  rewrite lookup_insert_ne //. destruct (M'!!a) as [[]|]; [| |done].
+  { subst F' K'. destruct HV. split~. unfolds fupdate. case_if~. }
+  { subst F'. auto. }
+Qed.
+
+(* [Mem] is preserved by installing a direct link from [x] to [y] during
+   path compression. *)
+
+Lemma Mem_compress : forall D F K F' M V x y,
+  Mem D F K V M ->
+  x \in D ->
+  F' = compress F x y ->
+  Mem D F' K V (<[x:=Link y]>M).
+Proof using.
+  introv HR Dx EG'. subst.
+  intros a Da. specializes HR Da. destruct (decide (x = a)) as [->|].
+  { rewrite lookup_insert. eauto using compress_x_z. }
+  { rewrite lookup_insert_ne //. destruct (M!!a) as [[]|];
+      [|by eauto using compress_preserves_other_edges|done].
+    destruct HR. split*.
+    eauto using compress_preserves_roots_other_than_x. }
+Qed.
+
+(* [Mem] is preserved when [V] is updated at one equivalence class and [M]
+   is updated at the representative element. *)
+
+Lemma Mem_update1 : forall D R F K M V r x v,
+  Inv D F K R V ->
+  Mem D F K V M ->
+  x \in D ->
+  r = R x ->
+  Mem D F K (update1 V R x v) (<[r := Root (K r) v]>M).
+Proof using.
+  introv HI HM E Rx. forwards* (Dr&Rr): Inv_root x r.
+  intros y Dy. specializes HM Dy. destruct (decide (r = y)) as [->|].
+  { rewrite lookup_insert. splits.
+    { applys* R_self_is_root. }
+    { done. }
+    { rewrite /update1 fcupdate_hit; congruence. } }
+  { rewrite lookup_insert_ne // /update1 /fcupdate. case_if~.
+    destruct~ (M!!y) as [[]|]; [|done..]. destruct HM as (H1&H2&H3).
+    forwards*: is_root_R_self H1. congruence. }
+Qed.
+
+(* -------------------------------------------------------------------------- *)
+
+(* Private lemmas about the representation predicate and about [mapsto_M]. *)
+
+
+Lemma mapsto_M_acc : forall M x c,
+  M !! x = Some c ->
+  mapsto_M M -∗ x ↦ val_of_content c ∗
+     (∀ c', x ↦ val_of_content c' -∗ mapsto_M (<[x:=c']>M)).
+Proof.
+  introv HM. iIntros "HM".
+  rewrite -[in mapsto_M _](insert_id _ _ _ HM) -insert_delete /mapsto_M.
+  rewrite big_sepM_insert ?lookup_delete //. iDestruct "HM" as "[$?]".
+  iIntros (?) "?". rewrite -insert_delete big_sepM_insert ?lookup_delete //.
+  iFrame.
+Qed.
+
+Lemma mapsto_M_acc_same : forall M x c,
+  M !! x = Some c ->
+  mapsto_M M -∗ x ↦ val_of_content c ∗ (x ↦ val_of_content c -∗ mapsto_M M).
+Proof.
+  introv HM. by apply (big_sepM_lookup_acc (λ _ _, _)).
+Qed.
+
+(* TODO : that should go into Iris libraries for big ops *)
+Lemma mapsto_M_union : forall M1 M2,
+  M1 ##ₘ M2 ->
+  mapsto_M M1 ∗ mapsto_M M2 ⊣⊢ mapsto_M (M1 ∪ M2).
+Proof.
+  introv HM12. unfold mapsto_M.
+  induction M1 as [|l x M1 ? IH] using map_ind.
+  { by rewrite big_opM_empty !left_id. }
+  rewrite -insert_union_l !big_sepM_insert //; last first.
+  { apply lookup_union_None; split; [done|]. specialize (HM12 l).
+    rewrite lookup_insert in HM12. revert HM12. case: (M2 !! l)=>//=. }
+  rewrite -assoc. f_equiv. apply IH. by eapply map_disjoint_insert_l.
+Qed.
+
+Lemma mapsto_M_insert : forall M x c,
+  M!!x = None ->
+  x ↦ val_of_content c ∗ mapsto_M M ⊣⊢ mapsto_M (<[x:=c]>M).
+Proof.
+  introv Mxc. rewrite /mapsto_M big_sepM_insert //.
+Qed.
+
+Lemma mapsto_M_disjoint : forall M1 M2,
+  mapsto_M M1 -∗ mapsto_M M2 -∗ ⌜ M1 ##ₘ M2 ⌝.
+Proof.
+  iIntros "* HM1 HM2" (x). unfold mapsto_M.
+  destruct (M1!!x) eqn:HM1, (M2!!x) eqn:HM2=>//.
+  iDestruct (big_sepM_lookup with "HM1") as "H1"=>//.
+  iDestruct (big_sepM_lookup with "HM2") as "H2"=>//.
+  by iDestruct (mapsto_valid_2 with "H1 H2") as %[].
+Qed.
+
+(* -------------------------------------------------------------------------- *)
+
+(* Public lemmas about the representation predicate. *)
+
+(* If [UF D R V] holds, then [R] is idempotent. *)
+
+Theorem UF_idempotent : forall D R V,
+  UF D R V -∗ ⌜ idempotent R ⌝.
+Proof using.
+  iDestruct 1 as (?????) "?". eauto 10 using idempotent_R.
+Qed.
+
+(* If [UF D R V] holds, then [R] preserves [D]. *)
+
+Theorem UF_image : forall D R V x, x \in D →
+  UF D R V -∗ ⌜ R x \in D ⌝.
+Proof using.
+  iDestruct 1 as (?????) "?". eauto 10 using sticky_R.
+Qed.
+
+(* If [UF D R V] holds, then [R] is the identity outside of [D]. *)
+
+Theorem UF_identity : forall D R V x, x \notin D ->
+  UF D R V -∗ ⌜ R x = x ⌝.
+Proof using.
+  iDestruct 1 as (?????) "?". eauto 10 using R_is_identity_outside_D.
+Qed.
+
+(* If [UF D R V] holds, then [V] is compatible with [R]. *)
+
+Theorem UF_compatible : forall D R V x, x \in D ->
+  UF D R V -∗ ⌜ V x = V (R x) ⌝.
+Proof using.
+  iDestruct 1 as (?????) "?". eauto.
+Qed.
+
+(* An empty instance of the Union-Find data structure can be created out of
+   thin air. This is how the data structure is initialized. *)
+
+Theorem UF_create : forall V,
+  TC_invariant ={⊤}=∗ UF \{} id V.
+Proof using.
+  unfold UF. iIntros (V) "#?".
+  iExists (@LibRelation.empty elem), (λ _, 0%nat), ∅.
+  repeat iSplitL.
+  { iPureIntro. constructors.
+    { apply is_rdsf_empty. }
+    { intro x. eapply is_repr_empty. }
+    { eauto. } }
+  { iIntros "!%" (??). false. }
+  { rewrite /mapsto_M. by auto. }
+  { rewrite Phi_empty. by iApply zero_TC. }
+Qed.
+
+(* Two separate instances of the UnionFind data structure can be merged, without
+   actually doing anything at runtime. *)
+
+(* In principle, we could also prove the converse property, [UF_split]. A UnionFind
+   data structure can be split in two independent parts, provided the split respects
+   the equivalence relation. Considering the amount of dreary work that went into
+   establishing [UF_join], I leave this to future work. *)
+
+Theorem UF_join : forall D1 R1 V1 D2 R2 V2,
+  UF D1 R1 V1 -∗ UF D2 R2 V2 -∗
+  UF
+    (D1 \u D2)
+    (fun x => If x \in D1 then R1 x else R2 x)
+    (fun x => If x \in D1 then V1 x else V2 x)
+  ∗ ⌜ D1 \# D2 ⌝.
+Proof using.
+  intros.
+  iDestruct 1 as (F1 K1 M1 HI1 HM1) "(HM1 & HTC1)".
+  iDestruct 1 as (F2 K2 M2 HI2 HM2) "(HM2 & HTC2)".
+  sets D: (D1 \u D2).
+  sets R: (fun x => If x \in D1 then R1 x else R2 x).
+  sets V: (fun x => If x \in D1 then V1 x else V2 x).
+  set (F := LibRelation.union F1 F2).
+  set (K := fun x => If x \in D1 then K1 x else K2 x).
+  set (M := M1 ∪ M2).
+
+  (* Disjointness lemmas. Trivial and painful. *)
+
+  iDestruct (mapsto_M_disjoint with "HM1 HM2") as %HM12.
+
+  assert (forall x, x \in D1 -> x \in D2 -> False).
+  { intros l Hl1%HM1 Hl2%HM2. specialize (HM12 l).
+    destruct (M1!!l) eqn:HM1l=>//. destruct (M2!!l) eqn:HM2l=>//. }
+
+  assert (D1 \# D2) by by rew_set.
+
+  assert (forall x, x \in D2 -> x \notin D1).
+  { intros. intro. eauto. }
+
+  assert (forall x y, F1 x y -> x \in D1).
+  { eauto with confined is_dsf. }
+
+  assert (forall x y, F2 x y -> x \in D2).
+  { eauto with confined is_dsf. }
+
+  assert (forall x, x \in D1 -> F1 x = F x).
+  { intros. subst F. extens; intros y.
+    unfold LibRelation.union; split; intros; try branches; eauto; false; eauto. }
+
+  assert (forall x, x \in D2 -> F2 x = F x).
+  { intros. subst F. extens; intros y.
+    unfold LibRelation.union; split; intros; try branches; eauto; false; eauto. }
+
+  assert (forall x, x \in D1 -> K1 x = K x).
+  { intros. subst K. simpl. cases_if~. }
+
+  assert (forall x, x \in D2 -> K2 x = K x).
+  { intros. subst K. simpl. cases_if~. false; eauto. }
+
+  assert (forall x, x \in D1 -> R1 x = R x).
+  { intros. subst R. simpl. cases_if~. }
+
+  assert (forall x, x \in D2 -> R2 x = R x).
+  { intros. subst R. simpl. cases_if~. false; eauto. }
+
+  assert (forall x, x \in D1 -> V1 x = V x).
+  { intros. subst V. simpl. cases_if~. }
+
+  assert (forall x, x \in D2 -> V2 x = V x).
+  { intros. subst V. simpl. cases_if~. false; eauto. }
+
+  assert (forall x, x \in D1 -> M1!!x = M!!x).
+  { intros x Hx%HM1. subst M. destruct (M1!!x) eqn:? =>//.
+    symmetry. by apply lookup_union_Some_l. }
+
+  assert (forall x, x \in D2 -> M2!!x = M!!x).
+  { intros x Hx%HM2. subst M. destruct (M2!!x) eqn:? =>//.
+    symmetry. by apply lookup_union_Some_r. }
+
+  iSplit; last done. iExists F, K, M.
+
+  iCombine "HTC1 HTC2" as "HTC".
+  rewrite -mapsto_M_union // -Nat.mul_add_distr_l (@Phi_join 1 _ D F K); eauto.
+  iFrame. iPureIntro. split.
+
+  (* Preservation of [Inv]. *)
+  { destruct HI1, HI2. constructor.
+    (* Preservation of [is_rdsf]. *)
+    { subst D F K. eapply is_rdsf_join; eauto. }
+    (* Preservation of the agreement between [R] and [F]. *)
+    { intros x. subst F R. simpl. cases_if.
+      (* Case: [x \in D1]. *)
+      { eapply is_repr_join_direct_1; eauto. }
+      (* Case: [x \notin D1]. *)
+      { eapply is_repr_join_direct_2; eauto. }
+    }
+    (* Preservation of the compatibility of [V]. *)
+    { intros x. subst V R. simpl. cases_if; [ | destruct (classic (x \in D2)) ].
+      (* Case: [x \in D1]. *)
+      { assert (R1 x \in D1). { eauto using sticky_R. }
+        cases_if. intuition eauto. }
+      (* Case: [x \in D2]. *)
+      { assert (R2 x \in D2). { eauto using sticky_R. }
+        cases_if. false; eauto. eauto. }
+      (* Case: [x \notin D1 \u D2]. *)
+      { assert (h: R2 x = x). { eapply R_is_identity_outside_D; eauto with is_dsf. }
+        rewrite h. cases_if. reflexivity. }
+    }
+  }
+
+  (* Preservation of [Mem]. *)
+  { intros x Dx. subst D. rewrite in_union_eq in Dx.
+    destruct Dx as [ Dx | Dx ].
+    { forwards : HM1 Dx. destruct (M1!!x) as [c|] eqn:EQM1=>//.
+      unfold is_root in *. rewrite (lookup_union_Some_l _ _ _ _ EQM1) //.
+      repeat match goal with h: forall_ x \in D1, _ |- _ =>
+        specializes h Dx; try rewrite <- h
+      end. done. }
+    { forwards : HM2 Dx. destruct (M2!!x) as [c|] eqn:EQM2=>//.
+      unfold is_root in *. rewrite (lookup_union_Some_r _ _ _ _ HM12 EQM2) //.
+      repeat match goal with h: forall_ x \in D2, _ |- _ =>
+        specializes h Dx; try rewrite <- h
+      end. done. } }
+Qed.
+
+(* -------------------------------------------------------------------------- *)
+
+(* Verification of [make]. *)
+
+(* The function call [make v] requires [UF D R V] as well as O(1) time credits.
+   It returns a new element [x], that is, [x] is not in [D]. It updates the
+   data structure to [UF D' R' V'], where:
+   1. [D'] is [D] extended with [x];
+   2. [R'] is [R];
+   3. [V'] is [V] extended with a mapping of [x] to [v]. *)
+
+Theorem make_spec : forall D R V v,
+  TC_invariant -∗
+  {{{ UF D R V ∗ TC 16 }}}
+    «make v»
+  {{{ (x : elem), RET #x;
+      let D' := D \u \{x} in
+      let V' := update1 V R x «v»%V in
+      UF D' R V' ∗
+      ⌜x \notin D /\
+       R x = x⌝ }}}.
+Proof using.
+  iIntros "* #?" (Φ) "!# [HF TC] HΦ". rewrite /= !translation_of_val.
+  wp_tick_rec. wp_tick. wp_alloc x as "Hx". iApply "HΦ".
+  iDestruct "HF" as (F K M HI HM) "[HM TC']".
+
+  iAssert ⌜M !! x = None⌝%I as %Mx.
+  { case HMx: (M!!x)=>//.
+    iDestruct (big_sepM_lookup with "HM") as "Hx'"=>//.
+    by iDestruct (mapsto_valid_2 with "Hx Hx'") as %[]. }
+  assert (x \notin D) as Dx.
+  { intros Dx%HM. by rewrite Mx in Dx. }
+
+  iSplit; [|by eauto 10 using R_is_identity_outside_D].
+  iExists _, _, (<[x:=Root 0 _]>M).
+  rewrite -Phi_extend 1?Nat.mul_add_distr_l; eauto; []. iCombine "TC' TC" as "$".
+  repeat iSplit; try iPureIntro.
+  { applys* Inv_make. } { applys* Mem_make. }
+  iApply mapsto_M_insert; [done|iFrame].
+Qed.
+
+(* -------------------------------------------------------------------------- *)
+
+(* Verification of [find]. *)
+
+(* Because [find] is a recursive function, we must begin with a specification
+   that is amenable to an inductive proof. It states that [find] essentially
+   implements the mathematical predicate [bw_ipc]. If [bw_ipc F x d F'] holds,
+   which means that path compression at [x] requires [d] steps and changes the
+   graph from [F] to [F'], then [find] requires [d+1] time credits and changes
+   the memory from [M] to some [M'] that agrees with [F']. Furthermore, the
+   value [r] returned by [find] is the representative of [x]. *)
+
+Lemma find_spec_inductive: forall d D R F K F' M V x,
+  Inv D F K R V ->
+  Mem D F K V M ->
+  x \in D ->
+  bw_ipc F x d F' ->
+  TC_invariant -∗
+  {{{ mapsto_M M ∗ TC (7*d+8) }}}
+    «find #x»
+  {{{ M', RET #(R x); mapsto_M M' ∗ ⌜ Mem D F' K V M' ⌝ }}}.
+Proof using.
+  intros d. rewrite /= translation_of_val /find. unlock. simpl.
+  induction_wf IH: Wf_nat.lt_wf d.
+  introv HI HM Dx HC. iIntros "#?" (Φ) "!# [HM TC] HΦ /=".
+  iDestruct "TC" as "[TCd TC]". wp_tick_rec.
+  assert (HV := HM _ Dx). destruct (M !! x) as [c|] eqn:? =>//.
+  iDestruct (mapsto_M_acc_same with "HM") as "[Hx HM]"=>//. wp_tick_load.
+  iDestruct ("HM" with "Hx") as "HM". destruct c as [k v|y].
+  (* Case: Root. *)
+  { wp_tick_match. wp_tick_proj. wp_tick_seq. wp_tick_proj. wp_tick_seq.
+    destruct HV as [HR HP]. forwards* EQ : is_root_R_self HR. rewrite EQ.
+    iApply "HΦ". iFrame. iPureIntro.
+    invert HC; intros. by subst. by false* a_root_has_no_parent HR.
+  }
+  (* Case: Link. *)
+  { wp_tick_match. rename HV into HF. invert HC.
+    { intros. subst F. subst. false* a_root_has_no_parent. }
+    intros F'0 F'' x0 y0 z' d' HF' HR' HB' EF' Ex Ed EF''. subst F'' x0 d.
+    lets* E: is_dsf_functional D HF HF'. subst y0. clear HF'.
+    assert (y \in D). { eauto with confined is_dsf. }
+    assert (z' = R y). { symmetry. eapply is_repr_incl_R; eauto. } subst z'.
+    forwards IH' : IH HI HM HB'; [math|done|].
+    iCombine "TCd TC" as "TC".
+    math_rewrite (7 * S d' + 4 = 7 * d' + 8 + 3)%nat.
+    iDestruct "TC" as "[TCd TC]".
+    (* FIXME : wp_apply does not work. *)
+    wp_bind (tick _ #y). iApply (IH' with "[//] [$HM $TCd]").
+    iIntros "!>" (M') "[HM' hM']". iDestruct "hM'" as %HM'. wp_tick_let.
+    assert (HV := HM' _ Dx). destruct (M' !! x) as [c|] eqn:? =>//.
+    iDestruct (mapsto_M_acc with "HM'") as "[Hx HM']"=>//.
+    wp_tick_store. wp_tick_seq.
+    iDestruct ("HM'" $! (Link (R y)) with "Hx") as "HM'".
+    assert (is_equiv F x y). { eauto using path_is_equiv with rtclosure. }
+    assert (R x = R y) as ->. { eauto using is_equiv_incl_same_R. }
+    iApply ("HΦ" with "[$HM']").
+    iPureIntro. applys~ Mem_compress HM'. }
+Qed.
+
+(* The function call [find x] requires [UF D R V] as well as O(alpha(D)) time
+   credits. It preserves [UF D R V] and returns the representative of [x]. *)
+
+Theorem find_spec : forall D R V x, x \in D ->
+  TC_invariant -∗
+  {{{ UF D R V ∗ TC (14 * alpha (card D) + 29) }}}
+    «find #x»
+  {{{ RET #(R x); UF D R V }}}.
+Proof using.
+  introv Dx. iIntros "#?" (Φ) "!# [UF TC1] HΦ".
+  iDestruct "UF" as (F K M HI HM) "[HM TC2]".
+  forwards* (d&F'&HC&HP): amortized_cost_of_iterated_path_compression_simplified x.
+  iCombine "TC1 TC2" as "TC".
+  rewrite [TC (_ + _)](TC_weaken _ (7*Phi D F' K + (7 * d + 8))%nat); [|math].
+  iDestruct "TC" as "[TC1 TC2]".
+  iApply (find_spec_inductive with "[//] [$TC2 $HM]")=>//.
+  iIntros "!>" (M') "[HM' %]". iApply "HΦ".
+  iExists _, _, _. iFrame. iPureIntro. split; [|done].
+  split; eauto 10 using is_rdsf_bw_ipc, bw_ipc_preserves_RF_agreement.
+Qed.
+
+(* -------------------------------------------------------------------------- *)
+
+(* Verification of [get]. *)
+
+(* The function call [get x] requires [UF D R V] as well as O(alpha(D)) time
+   credits. It preserves [UF D R V] and returns the data stored at [x]. *)
+
+Theorem get_spec : forall D R V x, x \in D ->
+  TC_invariant -∗
+  {{{ UF D R V ∗ TC (14 * alpha (card D) + 38) }}}
+    «get #x»
+  {{{ RET V x; UF D R V }}}.
+Proof using.
+  introv Dx. iIntros "#?" (Φ) "!# [UF TC] HΦ".
+  math_rewrite (14 * alpha (card D) + 38 = 14 * alpha (card D) + 29 + 9)%nat.
+  iDestruct "TC" as "[TC1 TC2]".
+  (* FIXME : all these rewrites should not appear. *)
+  rewrite /get. unlock. rewrite /= !translation_of_val. wp_tick_let.
+  rewrite -(translation_of_val find). wp_apply (find_spec with "[//] [$TC1 $UF]")=>//.
+  iIntros "UF". wp_tick_let. iDestruct "UF" as (F K M HI HM) "[HM TC]".
+  forwards* (Drx&Rrx): Inv_root x (R x).
+  forwards* EM: Mem_root (R x).
+  iDestruct (mapsto_M_acc_same with "HM") as "[Hx HM]"=>//. wp_tick_load.
+  iDestruct ("HM" with "Hx") as "HM".
+  wp_tick_match. wp_tick_proj. wp_tick_seq. wp_tick_proj. wp_tick_let.
+  rewrite -(Inv_data _ _ _ _ _ HI). iApply "HΦ".
+  iExists _, _, _. eauto with iFrame.
+Qed.
+
+
+(* -------------------------------------------------------------------------- *)
+
+(* Verification of [set]. *)
+
+(* The function call [set x v] requires [UF D R V] as well as O(alpha(D)) time
+   credits. It produces [UF D R V'], where [V'] is obtained from [V] by mapping
+   the equivalence class of [x] to [v]. *)
+
+Theorem set_spec : forall D R V x v,
+  x \in D ->
+  TC_invariant -∗
+  {{{ UF D R V ∗ TC (14 * alpha (card D) + 40) }}}
+    «set #x v»
+  {{{ RET #(); UF D R (update1 V R x «v»%V) }}}.
+Proof using.
+  introv Dx. iIntros "#?" (Φ) "!# [UF TC] HΦ".
+  math_rewrite (14 * alpha (card D) + 40 = 14 * alpha (card D) + 29 + 11)%nat.
+  iDestruct "TC" as "[TC1 TC2]".
+  (* FIXME : all these rewrites should not appear. *)
+  rewrite /set. unlock. rewrite /= !translation_of_val. wp_tick_let. wp_tick_let.
+  rewrite -(translation_of_val find). wp_apply (find_spec with "[//] [$TC1 $UF]")=>//.
+  iIntros "UF". wp_tick_let. iDestruct "UF" as (F K M HI HM) "[HM TC]".
+  forwards* (Drx&Rrx): Inv_root x (R x).
+  forwards* EM: Mem_root (R x).
+  iDestruct (mapsto_M_acc with "HM") as "[Hx HM]"=>//. wp_tick_load.
+  wp_tick_match. wp_tick_proj. wp_tick_seq. wp_tick_proj. wp_tick_seq. wp_tick_store.
+  iApply "HΦ". iExists _, _, _. iFrame.
+  iSplit; [auto using Inv_update1|]. iSplit; [eauto using Mem_update1|].
+  rewrite Rrx. by iApply "HM".
+Qed.
+
+(* -------------------------------------------------------------------------- *)
+
+(* Verification of [eq]. *)
+
+(* The function call [eq x y] requires [UF D R V] as well as O(alpha(D)) time
+   credits. It preserves [UF D R V] and returns a Boolean outcome which
+   indicates whether [x] and [y] are members of a common equivalence class. *)
+
+Theorem eq_spec : forall D R V x y,
+  x \in D -> y \in D ->
+  TC_invariant -∗
+  {{{ UF D R V ∗ TC (28 * alpha (card D) + 61) }}}
+    «eq #x #y»
+  {{{ RET #(bool_decide (R x = R y)); UF D R V }}}.
+Proof using.
+  introv Dx Dy. iIntros "#?" (Φ) "!# [UF TC] HΦ".
+  math_rewrite (28 * alpha (card D) + 61 =
+                (14 * alpha (card D) + 29) + (14 * alpha (card D) + 29) + 3)%nat.
+  iDestruct "TC" as "[[TC1 TC2] TC3]".
+  (* FIXME : all these rewrites should not appear. *)
+  rewrite /eq. unlock. rewrite /= !translation_of_val. wp_tick_let. wp_tick_let.
+  rewrite -(translation_of_val find).
+  wp_apply (find_spec with "[//] [$TC1 $UF]")=>//. iIntros "UF".
+  wp_apply (find_spec with "[//] [$TC2 $UF]")=>//. iIntros "UF".
+  wp_tick_op.
+  rewrite (bool_decide_iff (#(R x) = #(R y)) (R x = R y)); last (split; congruence).
+  by iApply "HΦ".
+Qed.
+
+
+(* -------------------------------------------------------------------------- *)
+
+(* Machine int addition with time credits. *)
+
+Lemma machine_int_add_spec_tc n1 n2 :
+  TC_invariant -∗
+  {{{ is_machine_int n1 ∗ is_machine_int n2 ∗ ⌜min_int ≤ n1+n2 < max_int⌝ ∗
+      TC 6 }}}
+    «machine_int_add #n1 #n2»
+  {{{ RET #(n1+n2) ; is_machine_int (n1+n2) }}}.
+Proof.
+  iIntros "#? !#" (Φ) "(_ & _ & % & TC) Post". rewrite /= translation_of_val.
+  wp_tick_rec. wp_tick_let. repeat wp_tick_op.
+  (* boring arithmetic proof: *)
+  assert ((n1 + n2 + max_int) `rem` max_uint - max_int = n1 + n2) as ->. {
+    assert ((n1 + n2 + max_int) `rem` max_uint = n1 + n2 + max_int). {
+      apply Z.rem_small. unfold min_int, max_uint in *. lia.
+    }
+    lia.
+  }
+  by iApply "Post".
+Qed.
+
+(* -------------------------------------------------------------------------- *)
+
+(* Verification of [link]. (This is an internal function.) *)
+
+(* The function call [link x y] requires [UF D R V] as well as O(1) time credits.
+   It requires [x] and [y] to be roots. It chooses the new representative [z] to
+   be one of [x] or [y], and returns [z], together with [UF D' R' V'], where:
+   1. [D'] is [D], i.e., the domain is unchanged;
+   2. [R'] is [R], where the equivalence classes of [x] and [y] are mapped to [z];
+   3. [V'] is [V], where the equivalence classes of [x] and [y] are mapped to [V z].
+*)
+
+Lemma link_spec : forall D R V x y,
+  x \in D ->
+  y \in D ->
+  R x = x ->
+  R y = y ->
+  TC_invariant -∗
+  {{{ UF D R V ∗ TC 46 }}}
+    «link #x #y»
+  {{{ z, RET #z; UF D (update2 R R x y z) (update2 V R x y (V z)) ∗
+                   ⌜z = x \/ z = y⌝}}}.
+Proof using.
+  introv Dx Dy Rx Ry. iIntros "#?" (Φ) "!# [UF TC] HΦ".
+  rewrite /link. unlock. rewrite /= !translation_of_val. wp_tick_let. wp_tick_let.
+  iDestruct "UF" as (F K M HI HM) "[HM TC']".
+  wp_tick_op. case_bool_decide as Hxy.
+  (* Case: [x == y]. *)
+  { inversion Hxy. subst. wp_tick_if. iApply "HΦ".
+    rewrite update2_R_self; [|by eauto]. erewrite update2_V_self; [|by eauto..].
+    iSplit; [|by auto]. iExists _, _, _. auto with iFrame. }
+  (* Case: [x != y]. *)
+  wp_tick_if.
+  forwards Hx: HM Dx. forwards Hy: HM Dy.
+  destruct (M !! x) as [cx|] eqn:EQx, (M !! y) as [cy|] eqn:EQy=>//.
+  iDestruct (mapsto_M_acc_same _ x with "HM") as "[Hx HM]"=>//.
+  wp_tick_load. iDestruct ("HM" with "Hx") as "HM".
+  destruct cx; wp_tick_match;
+    last by false; eauto using a_root_has_no_parent, R_self_is_root.
+  wp_tick_proj. wp_tick_let. wp_tick_proj. wp_tick_let.
+  iDestruct (mapsto_M_acc_same _ y with "HM") as "[Hy HM]"=>//.
+  wp_tick_load. iDestruct ("HM" with "Hy") as "HM".
+  destruct cy; wp_tick_match;
+    last by false; eauto using a_root_has_no_parent, R_self_is_root.
+  wp_tick_proj. wp_tick_let. wp_tick_proj. wp_tick_let.
+  destruct Hx as (HRx&Kx&Vx). substs. destruct Hy as (HRy&Ky&Vy). substs.
+  wp_tick_op; case_bool_decide; wp_tick_if;
+    [|wp_tick_op; case_bool_decide; wp_tick_if].
+  (* Sub-case: [K x < K y]. *)
+  { iDestruct (mapsto_M_acc _ x with "HM") as "[Hx HM]"=>//.
+    wp_tick_store. wp_tick_seq. iApply "HΦ". iSplit; [|by auto].
+    Inv_link
+    (* F' := *) (UnionFind03Link.link F x y)
+    (* K' := *) K
+    (* V' := *) (update2 V R x y (V y))
+                x y
+    (* z  := *) y.
+    iCombine "TC' TC" as "TC". iExists _, _, (<[x:=Link y]>M). iSplit; [done|].
+    rewrite TC_weaken; [iFrame "TC"|lia]. iSplit; [by eauto using Mem_link|].
+    by iApply "HM". }
+  (* Sub-case: [K x > K y]. *)
+  { iDestruct (mapsto_M_acc _ y with "HM") as "[Hy HM]"=>//.
+    wp_tick_store. wp_tick_seq. iApply "HΦ".
+    rewrite [update2 _ _ _ _ x]update2_sym. rewrite [update2 _ _ _ _ (V x)]update2_sym.
+    iSplit; [|by auto].
+    Inv_link
+    (* F' := *) (UnionFind03Link.link F y x)
+    (* K' := *) K
+    (* V' := *) (update2 V R y x (V x))
+                y x
+    (* z  := *) x.
+    iCombine "TC' TC" as "TC". iExists _, _, (<[y:=Link x]>M). iSplit; [done|].
+    rewrite TC_weaken; [iFrame "TC"|lia]. iSplit; [by eauto using Mem_link|].
+    by iApply "HM". }
+  (* Sub-case: [K x = K y]. *)
+  { iDestruct (mapsto_M_acc _ y with "HM") as "[Hy HM]"=>//.
+    wp_tick_store.
+    iDestruct ("HM" $! (Link _) with "Hy") as "HM".
+    wp_tick_seq.
+    rewrite -translation_of_val (_:22=6+16)%nat //.
+    iDestruct "TC" as "[TC1 TC2]".
+    wp_apply (machine_int_add_spec_tc with "[//] [$TC1]").
+    admit. iIntros "_". (* No overflow. *)
+    rewrite -(Nat2Z.inj_add _ 1).
+    iDestruct (mapsto_M_acc _ x with "HM") as "[Hx HM]".
+    { rewrite lookup_insert_ne //. congruence. }
+    wp_tick_store.
+    iDestruct ("HM" $! (Root _ _) with "Hx") as "HM".
+    wp_tick_seq.
+    iApply "HΦ". iSplit; [|by auto].
+    assert (K x = K y). { math. }
+    Inv_link
+    (* F' := *) (UnionFind03Link.link F y x)
+    (* K' := *) (fupdate K x (1 + K x)%nat)
+    (* V' := *) (update2 V R x y (V x))
+                x y
+    (* z  := *) x.
+    iExists _, _, _. iSplit; [done|]. iFrame "HM".
+    iCombine "TC' TC2" as "TC".
+    rewrite TC_weaken; [iFrame "TC"|lia].
+    iPureIntro. applys* Mem_link_incr HM. congruence. applys update2_sym.
+  }
+Admitted.
+
+(* -------------------------------------------------------------------------- *)
+
+(* Verification of [union]. *)
+
+(* The function call [union x y] requires [UF D R V] as well as O(alpha(D)) time
+   credits. It chooses the new representative [z] to be one of [x] or [y], and
+   returns [z], together with [UF D' R' V'], where:
+   1. [D'] is [D], i.e., the domain is unchanged;
+   2. [R'] is [R], where the equivalence classes of [x] and [y] are mapped to [z];
+   3. [V'] is [V], where the equivalence classes of [x] and [y] are mapped to [V z].
+*)
+
+Theorem union_spec : forall D R V x y,
+  x \in D ->
+  y \in D ->
+  TC_invariant -∗
+  {{{ UF D R V ∗ TC (28 * alpha (card D) + 106) }}}
+    «union #x #y»
+  {{{ z, RET #z; UF D (update2 R R x y z) (update2 V R x y (V z)) ∗
+                 ⌜z = R x \/ z = R y⌝ }}}.
+Proof using.
+  introv Dx Dy.
+  math_rewrite (28 * alpha (card D) + 106 =
+                (14 * alpha (card D) + 29) + (14 * alpha (card D) + 29) + 46 + 2)%nat.
+  iIntros "#?" (Φ) "!# [UF [[[TC1 TC2] TC3] TC4]] HΦ".
+  rewrite /union. unlock. rewrite /= !translation_of_val. wp_tick_let. wp_tick_let.
+  rewrite -[in App _ #y]translation_of_val.
+  wp_apply (find_spec with "[//] [$TC1 $UF]")=>//. iIntros "UF".
+  rewrite -[in App _ #x]translation_of_val.
+  wp_apply (find_spec with "[//] [$TC2 $UF]")=>//. iIntros "UF".
+  rewrite -translation_of_val.
+  iDestruct (UF_image _ _ _ x with "UF") as %? =>//.
+  iDestruct (UF_image _ _ _ y with "UF") as %? =>//.
+  iDestruct (UF_idempotent with "UF") as %Idem =>//.
+  wp_apply (link_spec with "[//] [$TC3 $UF]")=>//.
+  iIntros (z). by rewrite !update2_root.
+Qed.
+
+End UnionFind.
+
+(* Print Assumptions UF_idempotent. *)
+(* Print Assumptions UF_image. *)
+(* Print Assumptions UF_identity. *)
+(* Print Assumptions UF_compatible. *)
+(* Print Assumptions UF_create. *)
+(* Print Assumptions UF_join. *)
+(* Print Assumptions make_spec. *)
+(* Print Assumptions find_spec. *)
+(* Print Assumptions get_spec. *)
+(* Print Assumptions set_spec. *)
+(* Print Assumptions eq_spec. *)
+(* Print Assumptions union_spec. *)
